\chapter{Trigonometry}
\section{Sine, Cosine, and Tangent}
\begin{figure}[H]
  \begin{center}
    \includegraphics[width=0.4\textwidth]{continuous/trig/basictrig}
  \end{center}
  \caption{A right triangle.}
  \label{fig:right_triangle}
\end{figure}
\begin{defn}
    The \textbf{hypotenuse}\index{hypotenuse} is the side opposite the right angle.
\end{defn}
\begin{defn}
    The \textbf{sine}\index{sine} of $theta$, $\sin\theta$, is equal to the length of the opposite side divided by the length of the hypotenuse.
\end{defn}
\begin{defn}
    The \textbf{cosine}\index{cosine} of $theta$, $\cos\theta$, is equal to the adjacent side divided by the hypotenuse.
\end{defn}
\begin{defn}
    The \textbf{tangent}\index{tangent} of $theta$, $\tan\theta$, is equal to the opposite over the adjacent side.
\end{defn}
In \figref{fig:right_triangle}:
  \[\displaystyle{\sin\theta=\frac{b}{c}}\qquad
  \displaystyle{\cos\theta=\frac{a}{c}}\qquad
  \displaystyle{\tan\theta=\frac{b}{a}}\]

\input{continuous/unitcircle}

\section{Trigonometric Identities}\index{trigonometric identities}
Our first pythagorean identity is just derived from the pythagorean theorem.
\begin{theorem}
  In any right triangle, the area of the square whose side is the hypotenuse (the side opposite the right angle) is equal to the sum of the areas of the squares whose sides are the two legs (the two sides that meet at a right angle).
  %credit: wikipedia. Anyone have a better source?
  \label{th:pythagoras}
\end{theorem}
\begin{figure}[h]
  \begin{center}
    \subfigure[The Pythagorean Theorem states that the sum of the areas square $a$ and square $b$ is equal to the area of square $c$.]{\
      \includegraphics[width=0.4\textwidth]{continuous/functions/pyth}
      \label{fig:pyth}
    }
    \hspace{0.1\textwidth}
    \subfigure[The equation for a unit circle is $a^2+b^2=1$. This creates a circle with a radius of $1$.]{\
      \includegraphics[width=0.4\textwidth]{continuous/functions/unitcirc}
      \label{fig:basicuniticircle}
    }
  \end{center}
\end{figure}
\begin{figure}[h]
  \begin{center}
    \includegraphics[width=0.5\textwidth]{continuous/trig/pythcircle}
    \caption{The pythagorean squares on a unit circle. Note that the length of side $c$ must be $1$ because the radius of the circle is $1$.}
  \end{center}
  \label{fig:pythcircle}
\end{figure}
Because the radius of the circle is $1$, then the length of side $c$ must also equal $1$.
From this, we can conclude that $\sin^2x+\cos^2x$ must, indeed, equal 1.

Why? From the picture, it is clear that both $c$ and $r$ are equal to $1$. Using the pythagorean theorem (\thref{th:pythagoras}):
\begin{proof}\begin{align*}
  a^2+b^2&=c^2\\
  a\cdot a + b \cdot b &= c \cdot c \\
  \intertext{we divide both sides by 1}
  \frac{b}{1}\cdot\frac{b}{1}+\frac{a}{1}\cdot\frac{a}{1}
  &=\frac{c \cdot c}{1}\\
  \intertext{because $c=1$}
  \frac{b}{c}\cdot\frac{b}{c}+\frac{a}{c}\cdot\frac{a}{c}
  &=1\\
  \intertext{remembering our definitions of sine and cosine}
  \sin\theta \cdot \sin\theta + \cos\theta \cdot \cos\theta &=1\\
  \sin^2\theta + \cos^2\theta &=1\qedhere
\end{align*}\end{proof}
We now have our first trigonometric identity.
\begin{equation}
  \sin^2x+\cos^2x=1
  \label{eq:pythtrig}
\end{equation}
The other ones, we either have to memorize or learn to derive (described in \secref{sec:trigderiv}).
\begin{equation}
  \sin{(x+y)} = \sin x \cos y + \sin y \cos x
\end{equation}
\begin{equation}
  \sin{(x-y)} = \sin x \cos y - \sin y \cos x
\end{equation}
\begin{equation}
  \cos(x+y)=\cos x \cos y - \sin x \sin y
  \label{eq:cosxpy}
\end{equation}
\begin{equation}
  \cos(x-y)=\cos x \cos y + \sin x \sin y
\end{equation}
\begin{equation}
  \sin{-x}=-\sin x
\end{equation}
\begin{equation}
  \sin{-x}=-\sin x
\end{equation}
\begin{equation}
  \sin{2x}=2 \big( \sin x \cos x \big)
\end{equation}
\begin{equation}
  \cos{2x}=\cos^2x-\sin^2x
\end{equation}

\section{Reciprocal functions}\index{reciprocal trigonometric functions}
The reciprocals of $\sin$, $\cos$, and $\tan$ all have names as well:
\begin{defn}
    The \textbf{cosecant}, $\csc \theta$ is the reciprocal of $\sin \theta$:
    \begin{equation}
        \csc \theta = \frac{1}{\sin \theta}
        \label{eq:cosecant}
    \end{equation}
\end{defn}
\begin{defn}
    The \textbf{secant}, $\sec \theta$ is the reciprocal of $\csc \theta$:
    \begin{equation}
        \sec \theta = \frac{1}{\cos \theta}
        \label{eq:secant}
    \end{equation}
\end{defn}
\begin{defn}
    The \textbf{cotangent}, $\cot \theta$ is the reciprocal of $\tan \theta$:
    \begin{equation}
        \cot \theta = \frac{1}{\tan \theta}
        \label{eq:cotangent}
    \end{equation}
\end{defn}

\section{Deriving Trigonometric Identities}\index{deriving trigonometric identities}\label{sec:trigderiv}
Recall in \figref{fig:right_triangle}, $\sin \theta = b/c$ and $\cos \theta = a/c$.
Therefore,
\begin{equation*}
    \frac{\sin \theta}{\cos \theta} = \dfrac{b/c}{a/c},
\end{equation*}
which we may simplify into
\begin{equation*}
    \frac{\sin \theta}{\cos \theta} = \dfrac{bc}{ac},
\end{equation*}
and cancel like terms to get
\begin{equation*}
    \frac{\sin\theta}{\cos\theta}=\dfrac{b}{a}.
\end{equation*}
Recall that $\tan \theta = b/a$ and we see that
\begin{equation}
    \tan\theta = \frac{\sin \theta}{\cos \theta}.
    \label{eq:found_tangent}
\end{equation}
Now, taking the reciprocal of both sides of \eref{eq:found_tangent}:
\begin{equation*}
    \frac{1}{\tan \theta} = \frac{\cos \theta}{\sin \theta}.
\end{equation*}
Finally, remembering \eref{eq:cotangent},
\begin{equation}
    \cot \theta = \frac{\cos \theta}{\sin \theta}.
    \label{eq:found_cotangent}
\end{equation}

We recall that using the pythagorean theorem and a triangle with a hypotenuse of length $1$, we can obtain \eref{eq:pythtrig}:
\begin{equation*}
	\sin^2x+\cos^2x=1.
\end{equation*}
Dividing by $\sin^2x$ gives us:
\begin{align*}
    \frac{\sin^2x}{\sin^2x}+\frac{\cos^2x}{\sin^2x} &= \frac{1}{\sin^2x}, \\
    1+\cot^2x &= \csc^2x,
\end{align*}
and dividing by $\cos^2x$, we see that
\begin{align}
    \frac{\sin^2x}{\cos^2x}+\frac{\cos^2x}{\cos^2x}+=&\frac{1}{\cos^2x}, \nonumber \\
    \tan^2x+1=&\sec^2x.
\end{align}

We should memorize the following two identities:
\begin{equation}
  \sin{a+b}=\sin a \cos a + \sin b \cos b,
  \label{eq:sinab}
\end{equation}
and
\begin{equation}
  \cos{a+b}=\cos a \cos b + \sin a \sin b.
  \label{eq:cosab}
\end{equation}
From equation \eqref{eq:sinab} we can infer that if both $a$ and $b$ are the same then
\begin{equation}
  \sin{2\theta}=2 \sin \theta \cos \theta,
  \label{eq:sin2q}
\end{equation}
and using the same reasoning, \eqref{eq:cosab} gives us
\begin{align}
  \cos{2\theta}&=\cos \theta \cos \theta- \sin\theta \sin\theta, \nonumber\\
  \cos{2\theta}&=\cos^2 \theta - \sin^2\theta.
  \label{eq:cos2q}
\end{align}

We can generalize the pythagorean theorem by deriving the \textbf{law of cosines}\index{law of cosines}:
\begin{figure}[H]
  \begin{center}
    \includegraphics[width=0.4\textwidth]{continuous/trig/lawcosines}
  \end{center}
\end{figure}
In the above figure, we use the distance formula
\begin{equation}
  d=\sqrt{(x_1 - x_2)^2+(y_1-y_2)^2}
  \label{eq:distance}
\end{equation}
\begin{align}
  \notag  c &= \sqrt{(b-a\cos \theta)^2+(0-a\sin\theta)^2} \\
  \notag  c&=\sqrt{(b-a\cos\theta)^2+(a\sin\theta)^2} \\
  \notag  c^2&=(b-a\cos\theta)^2+(a\sin\theta)^2 \\
  \notag  c^2 &= (b-a\cos\theta)(b-a\cos\theta)+(a\sin\theta)(a\sin\theta) \\
  \notag  c^2 &= b^2 -ab\cos\theta -ab\cos\theta+(a\cos\theta)^2+(a\sin\theta)^2\\
  \notag  c^2&=b^2-2ab\cos\theta+(a\cos\theta)^2+(a\sin\theta)^2\\
  \intertext{Now we use the distance formula to find the length of $a$,}
  \notag  a&=\sqrt{(a\cos\theta)^2+(a\sin\theta)^2}\\
  \intertext{and square our result}
  \notag  a^2&=(a\cos\theta)^2+(a\sin\theta)^2\\
  \intertext{which now substitutes nicely into our original equation}
  \notag  c^2&=b^2-2ab\cos\theta+(a\cos\theta)^2+(a\sin\theta)^2\\
  \notag  c^2&=b^2-2ab\cos\theta+a^2\\
  c^2&=a^2+b^2-2ab\cos\theta
\end{align}
This is the \emph{law of cosines}\index{law of cosines},
a general form of the pythagorean theorem
that works with more than just right triangles.

By rearranging \eqref{eq:cos2q} and substituting from \eqref{eq:pythtrig} we can derive power reduction identities for $\cos^2 \theta$
\begin{align}
  \cos{2\theta} &= \cos^2 \theta - \sin^2\theta \nonumber \\
  \cos{2\theta} + \sin^2\theta &= \cos^2\theta \nonumber \\
  \cos{2\theta} + (1-\cos^2 \theta) &=\cos^2\theta \nonumber \\
  \cos{2\theta} + 1 &= \cos^2\theta + \cos^2\theta \nonumber \\
  \cos{2\theta}+1 &= 2 \cos^2\theta \nonumber \\
  \cos^2\theta &= \frac{\cos{2\theta}+1}{2}
  \label{eq:cossqq}
\end{align}
and for $\sin^2 \theta$
\begin{align}
  \cos{2\theta} &= \cos^2 \theta - \sin^2\theta \nonumber \\
  \sin^2 \theta &= \cos^2 \theta - \cos{2 \theta} \nonumber \\
  \sin^2 \theta &= (1-\sin^2 \theta) - \cos{2 \theta} \nonumber \\
  2 \sin^2 \theta &= 1-\cos{2\theta} \nonumber \\
  \sin^2 \theta &= \frac{1-\cos{2\theta}}{2}
  \label{eq:sinsqq}
\end{align}

\subsection{Examples}
\begin{ex}
  Find the value of
  \[ \cos{\frac{11 \pi}{12}} \text{.}\]
  \begin{sol}
    We first rewrite the problem to fit one of our trigonometric identities,
    then use equation \eqref{eq:cosxpy} to break apart $\cos{(11\pi /12)}$.
    \begin{align*}
      \cos{\frac{11 \pi}{12}}
      &=\cos{\frac{\pi}{4}+\frac{2 \pi}{3}}\\
      &=\cos{\frac{\pi}{4}} \cos{\frac{2\pi}{3}}
        -\sin\frac{\pi}{4} \sin\frac{2\pi}{3} \\
      \intertext{Unlike in the original problem, we can easily simplify our new expression.}
      &=\cos{\frac{\pi}{4}} \cos{\frac{2\pi}{3}}
        - \sin{\frac{\pi}{4}} \sin{\frac{2\pi}{3}}\\
      &= \frac{\sqrt 2}{2} \frac{-1}{2}
        -\frac{\sqrt 2}{2} \frac{\sqrt 3}{2}\\
      &=\frac{-\sqrt 2}{4}
        - \frac{\sqrt{6}}{4} \\
      &= \frac{-\sqrt 2}{4}\bigg(1+\sqrt 3\bigg)
    \end{align*}
  \end{sol}
\end{ex}
\begin{ex}
  Prove the following trigonometric identity:
  \[ \frac{1-\cos x}{\sin x}=\frac{\sin x}{1+\cos x} \]
  \begin{proof}
    We first cross-multiply:
    \begin{align*}
      \ (1-\cos x)(1+\cos x) &= sin^2 x \\
      \intertext{then, using equation \eqref{eq:pythtrig}, we realize that we can replace \(\sin^2 x\) with \(1-\cos^2 x\).}
       (1-\cos x)(1+\cos x) &= 1-\cos^2x\\
      \intertext{Now we simplify.}
      1-\cos x + \cos x -\cos^2 &= 1-\cos^2x \\
      1-\cos^2x &= 1-\cos^2x \qedhere
    \end{align*}
  \end{proof}
\end{ex}
\begin{figure}[h]
  \begin{center}
    \includegraphics[width=0.4\textwidth]{photos/pythagoras.jpg}
    \end{center}
    \caption{\emph{Busto di Pitagora. Copia romana di originale greco. Musei Capitolini, Roma}.
    Original uploader was \emph{Galilea} at \url{http://de.wikipedia.org}.
    File used under the terms of the Creative Commons Attribution-Share Alike 3.0 Unported license.}
  \label{fig:bustofpythagoras}
\end{figure}
